deps/poulet4/lib/P4automata/Combinators.v
@@ -1,23 +1,23 @@
 Require Import Poulet4.P4automata.P4automaton.
 Require Import Coq.Lists.List.
 
-Definition concat (l: p4automaton) (r: p4automaton) (r_start: states r) : p4automaton :=
+Program Definition concat (l: p4automaton) (r: p4automaton) (r_start: states r) : p4automaton :=
   {|
     store := store l * store r ;
-    states := states l + states r ; 
+    states := states l + states r ;
     size := fun s =>
       match s with
       | inl ls => l.(size) ls
       | inr rs => r.(size) rs
       end ;
-    update := fun st bs '(s_l, s_r) => 
+    update := fun st bs '(s_l, s_r) =>
       match st with
       | inl st' => (l.(update) st' bs s_l, s_r)
       | inr st' => (s_l, r.(update) st' bs s_r)
       end ;
-    transitions := fun st '(s_l, s_r) => 
-      match st with 
-      | inl st' => 
+    transitions := fun st '(s_l, s_r) =>
+      match st with
+      | inl st' =>
         match l.(transitions) st' s_l with
         | inl st'' => inl (inl st'')
         | inr true => inl (inr r_start)
@@ -30,20 +30,25 @@ Definition concat (l: p4automaton) (r: p4automaton) (r_start: states r) : p4auto
         end
       end ;
   |}.
+Next Obligation.
+  destruct s.
+  - apply l.
+  - apply r.
+Qed.
 
-Definition concat_config_l 
-  {l r: p4automaton} {r_start store_r} 
-  (c: configuration l) : configuration (concat l r r_start) := 
-  let '(state, store_l, bs) := c in 
+Definition concat_config_l
+  {l r: p4automaton} {r_start store_r}
+  (c: configuration l) : configuration (concat l r r_start) :=
+  let '(state, store_l, bs) := c in
   match state with
   | inl st => (inl (inl st), (store_l, store_r), bs)
   | inr b => (inr b, (store_l, store_r), bs)
   end.
 
-Definition concat_config_r 
-  {l r: p4automaton} {r_start store_l} 
-  (c: configuration r) : configuration (concat l r r_start) := 
-  let '(state, store_r, bs) := c in 
+Definition concat_config_r
+  {l r: p4automaton} {r_start store_l}
+  (c: configuration r) : configuration (concat l r r_start) :=
+  let '(state, store_r, bs) := c in
   match state with
   | inl st => (inl (inr st), (store_l, store_r), bs)
   | inr b => (inr b, (store_l, store_r), bs)
